

1. Consider the boundary value problem (12.1)-(12.2) with $f(x) = 1/x$. Using (12.3) prove that $u(x) = -x \log(x)$. This shows that $u \in C^2(0,1)$ but $u(0)$ is not defined and u', u'' do not exist at $x = 0$ (\Rightarrow : if $f \in C^0(0,1)$, but not $f \in C^0([0,1])$, then u does not belong to $C^0([0,1])$).

<Pf> by (12.3) the solution of boundary value problem is

$$u(x) = \int_0^1 G(x,s) f(s) ds, \text{ where } G(x,s) \text{ is Green's function}$$

$$\text{Let } f(x) = \frac{1}{x}$$

$$\begin{aligned} \Rightarrow u(x) &= \int_0^1 G(x,s) \cdot \frac{1}{s} ds \\ &= \int_0^x S(1-x)f(s) ds + \int_x^1 x(1-s)f(s) ds \\ &= \int_0^x S(1-x) \cdot \frac{1}{s} ds + \int_x^1 x(1-s) \frac{1}{s} ds \\ &= (1-x) \int_0^x \frac{1}{s} ds + x \int_x^1 \left(\frac{1}{s} - 1 \right) ds \\ &= (1-x) \cdot s \Big|_0^x + x \left(\ln s - s \right) \Big|_x^1 \\ &= (1-x) \cdot x - 0 + x \left[(0-1) - (\ln x - x) \right] \\ &= x - x^2 + x \left[-1 - \ln x + x \right] \\ &= x - x^2 - x - x \ln x + x^2 = -x \ln x, \end{aligned}$$

So $u(0)$ is not defined, also $u'(x) = -\ln x - 1$, $u''(x) = -\frac{1}{x}$

where $u'(0)$, $u''(0)$ is also not defined

6. Prove that $G^k(x_j) = hG(x_j, x_k)$, where G is Green's function introduced in (12.4) and G^k is its corresponding discrete counterpart of (12.4).

[Solution: we prove the result by verifying that $L_h G = h e^k$. Indeed, for a fixed x_k the function $G(x_k, s)$ is a straight line on the intervals $[0, x_k]$ and $[x_k, 1]$ so that $L_h G = 0$ at every node x_l with $l = 0, \dots, k-1$ and $l = k+1, \dots, n+1$. Finally, a direct computation shows that $(L_h G)(x_k) = 1/h$ which concludes the proof.]

7. Let u and v be functions that $T_h(u) = 1/h$ and $T_h(v) = 0$.

<P.f> for fixed x_k the function $G(x_k, s) = \begin{cases} s(1-x_k) & s \leq x_k \\ x_k(1-s) & s \geq x_k \end{cases}$

is a straight line in $[0, x_k]$ and $[x_k, 1]$

$$\text{So } L_h G(x_k, x_j) = \frac{G(x_k, x_{j-1}) - 2G(x_k, x_j) + G(x_k, x_{j+1}))}{h^2}$$

for x_j, x_{j+1}, x_{j-1} in one of the interval $[0, x_k]$ or $[x_k, 1]$

and $j \neq k$ we have

$$\begin{aligned} G(x_k, x_{j-1}) &= x_{j-1}(1-x_k), \quad G(x_k, x_{j+1}) = x_{j+1}(1-x_k), \quad G(x_k, x_j) = x_j(1-x_k) \\ &= (x_j-h)(1-x_k) \qquad \qquad \qquad = (x_j+h)(1-x_k) \end{aligned}$$

$$\Rightarrow G(x_k, x_{j-1}) - 2G(x_k, x_j) + G(x_k, x_{j+1})$$

$$= (x_j-h)(1-x_k) - 2x_j(1-x_k) + (x_j+h)(1-x_k)$$

$$= (1-x_k) [x_j-h - 2x_j + x_j+h] = 0$$

if $j = k$

$$L_h G(x_k, x_j) = -\frac{G(x_k, x_{k-1}) - 2G(x_k, x_k) + G(x_k, x_{k+1}))}{h^2}$$

$$\begin{aligned} G(x_k, x_{k-1}) &= x_{k-1}(1-x_k), \quad G(x_k, x_k) = x_k(1-x_k), \quad G(x_k, x_{k+1}) = x_k(1-x_{k+1}) \\ &= (x_k-h)(1-x_k) \qquad \qquad \qquad = x_k(1-(x_k+h)) \end{aligned}$$

$$\Rightarrow G(x_k, x_{k-1}) - 2G(x_k, x_k) + G(x_k, x_{k+1})$$

$$= (x_k-h)(1-x_k) - 2x_k(1-x_k) + x_k(1-x_k-h)$$

$$= (1-x_k)(-h-x_k) + x_k(1-x_k-h)$$

$$= -h + h\cancel{x_k} - \cancel{x_k}^2 + \cancel{x_k}^2 + x_k - \cancel{x_k}^2 - \cancel{x_k}h = -h$$

$$\therefore L_h G(x_k, x_k) = -\frac{-h}{h^2} = \frac{1}{h} \quad \Rightarrow \quad L_h G(x_k, x_j) = \begin{cases} \frac{1}{h} & \text{if } j=k \\ 0 & \text{if } j \neq k \end{cases}$$

define $\tilde{G}_1^k(x_j) = h G(x_j, x_k) \Rightarrow (L_h \tilde{G}_1^k)(x_j) = h (L_h G(x_j, x_k)) = \begin{cases} 1 & \text{if } j=k \\ 0 & \text{if } j \neq k \end{cases} = e^k$

and $\tilde{G}_1^k(x_0) = h G(x_0, x_k) = h G(x_n, x_k) = \tilde{G}_1^k(x_n) = 0$

$\therefore \tilde{G}_1^k(x_j)$ satisfy the same boundary value problem with G^k

$\therefore \tilde{G}_1^k(x_j) = G_1^k(x_j) = h G(x_j, x_k).$

2. check for any sequence $\{w_j\}_{j=0}^n$ and $\{v_j\}_{j=0}^n$ we have

$$\sum_{j=0}^{n-1} (w_{j+1} - w_j) v_j = w_n v_{n-1} - w_0 v_0 - \sum_{j=1}^{n-1} w_j (v_j - v_{j-1})$$

$$\langle \text{P.f.} \rangle \sum_{j=0}^{n-1} (w_{j+1} - w_j) v_j = \sum_{j=0}^{n-1} w_{j+1} v_j - \sum_{j=0}^{n-1} w_j v_j$$

$$\text{for } \sum_{j=0}^{n-1} w_{j+1} v_j, \text{ Let } i = j+1$$

$$\Rightarrow \sum_{i=1}^n w_i v_{i-1} = w_n v_{n-1} + \sum_{i=1}^{n-1} w_i v_{i-1} = w_n v_{n-1} + \sum_{j=1}^{n-1} w_j v_{j-1} \quad (1)$$

$$\text{for } \sum_{j=0}^{n-1} w_j v_j = w_0 v_0 + \sum_{j=1}^{n-1} w_j v_j \quad (2)$$

$$\Rightarrow (1) - (2) \Rightarrow w_n v_{n-1} + \sum_{j=1}^{n-1} w_j v_{j-1} - w_0 v_0 - \sum_{j=1}^{n-1} w_j v_j$$

$$= w_n v_{n-1} - w_0 v_0 + \sum_{j=1}^{n-1} w_j (v_{j-1} - v_j)$$

$$= w_n v_{n-1} - w_0 v_0 - \sum_{j=1}^{n-1} w_j (v_j - v_{j-1}) \neq$$

We want to show that $(L_h v_n, v_n)_h = h^{-1} \sum_{j=0}^{n-1} (v_{j+1} - v_j)^2$

$\langle \text{P.f.} \rangle$ By the def of inner product $(u, v)_h = h \sum_{j=1}^{n-1} u_j v_j$

$$\text{also } L_h v_n = - \frac{v_{j-1} - 2v_j + v_{j+1}}{h^2} = - \frac{(v_{j+1} - v_j) - (v_j - v_{j-1}))}{h^2}$$

$$\therefore (L_h v_n, v_n)_h = h \sum_{j=1}^{n-1} \left(- \frac{(v_{j+1} - v_j) - (v_j - v_{j-1}))}{h^2} \right) v_j$$

$$= - \frac{1}{h} \left[\sum_{j=1}^{n-1} (v_{j+1} - v_j) v_j - \sum_{j=1}^{n-1} (v_j - v_{j-1}) v_j \right]$$

$$\text{Let } a_j = v_{j+1} - v_j$$

$$(L_h v_n, v_n)_h = - \frac{1}{h} \left[\underbrace{\sum_{j=1}^{n-1} a_j v_j}_{S_1} - \underbrace{\sum_{j=1}^{n-1} a_{j-1} v_j}_{S_2} \right]$$

$$\because v_0 = 0$$



$$\text{for } S_1 = \sum_{j=1}^{n-1} a_j v_j = \sum_{j=0}^{n-1} a_j v_j \quad \because v_n = 0$$

$$\text{for } S_2 = \sum_{j=1}^{n-1} a_{j-1} v_j = \sum_{k=0}^{n-2} a_k v_{k+1} = \sum_{k=0}^{n-1} a_k v_{k+1}$$

$$\therefore S_1 - S_2 = \sum_{j=0}^{n-1} a_j v_j - \sum_{j=0}^{n-1} a_j v_{j+1} = \sum_{j=0}^{n-1} a_j (v_j - v_{j+1}) = - \sum_{j=0}^{n-1} (a_j)^2$$

$$\therefore (L_h v_n, v_n)_h = - \frac{1}{h} \sum_{j=0}^{n-1} (a_j)^2 = \frac{1}{h} \sum_{j=0}^{n-1} (v_{j+1} - v_j)^2 \neq$$